Working zero_neutral

Naturals.v
@@ -2,10 +2,10 @@
 Require Import Basics.
 Require Import Reduction.
 
-Fixpoint church_nat_aux (n: nat) (f: term): term :=
+Fixpoint church_nat_aux (n: nat): term :=
   match n with
-  | 0 => Var 0
-  | S n' => App f (church_nat_aux n' f)
+  | 0 => #0
+  | S n' => $ (#1) (church_nat_aux n')
   end
 .
 
@@ -20,7 +20,7 @@ End test_church_nat. *)
 
 (* Church encoding of a given natural *)
 Definition church_nat (n: nat): term :=
-  \\(church_nat_aux n (#1))
+  \\(church_nat_aux n)
 .
 
 Record term_nat := {
@@ -40,90 +40,306 @@ Qed.
 
 (* TODO fix this notation? *)
 Definition church_succ: term :=
-  \\\ App (#1) (App (App (#2) (#1)) (#0))
+  \\\ $ (#1) ($ ($ (#2) (#1)) (#0))
 .
 
 (* apply CTrans with (x' := p);
 [ apply CStep; unfold beta_step; simpl; now left | ]. *)
 
-Lemma church_succ_respects_nat (n: nat): $ church_succ (church_nat n) == church_nat (S n).
+(* Lemma replace_lemma (n: nat): $ (\ (\ church_nat_aux n)) (# 1) == \ church_nat_aux n.
 Proof.
   induction n.
-  - common_reduct.
-  - next_reduct (\\ App (#1) (App (App (church_nat (S n0)) (#1)) (#0))).
-    unfold church_nat.
-    apply CTrans with (x' := (\\ $ (# 1) $ (\ church_nat_aux (S n0) (# 1)) (# 0))).
-    + apply CStep.
-      unfold beta_step.
-      (* simpl. *) (* This kills the Coq *)
-
-    next_reduct (\\ $ (# 1) $ (\ church_nat_aux (S n0) (# 1)) (# 0)).
-    Compute beta_reducts (\ (\ $ (# 1) $ $ (\ (\ (#999))) (# 1) (# 0))).
-    (* Maybe RHS can be reduced a bit further? *)
-
-    (* LHS is equiv to: *)
-    (* next_reduct (\\ $ (# 1) (church_nat_aux (S n0) (# 1))). *)
-    (* which cannot be beta-reduced any further. *)
-
-    unfold church_nat.
-    destruct (S (S n0)).
-
-    apply CTrans with (x' := \\ $ (# 1) (church_nat_aux (S n0) (# 1)));
-    [ apply CStep|].
-    next_reduct (\\ $ (# 1) (church_nat_aux (S n0) (# 1))).
-    next_reduct (\\ church_nat_aux (S (S n0)) (# 1)).
-    next_reduct (\\ (App (# 1) (church_nat_aux (S n0) (# 1))) (# 1)).
+  (* TODO do base case! *)
+  Focus 2.
+  unfold church_nat_aux; fold church_nat_aux. *)
 
 
-  next_reduct $ (\ (\ (\ $ (# 1) $ $ (# 2) (# 1) (# 0)))) (\ (\ church_nat_aux n (# 1))).
+Fixpoint abstractionless (p: term): Prop :=
+  match p with
+  | #n => True
+  | \q => False
+  | $ q r => (abstractionless q) /\ (abstractionless r)
+  end
+.
+Require Import Coq.Arith.EqNat.
+
+Compute beta $ (\ #23) (#0) PRoot.
+
+(* Lemma eta_lemma (p: term) (_: abstractionless p) (n: nat): replace p (#n) n = p.
+Proof.
+  induction p.
+  - unfold replace.
+    destruct (EqNat.eq_nat_decide n n0).
+    + f_equal.
+      unfold increase_free_variables.
+      destruct (Compare_dec.le_lt_dec 0 n).
+      * 
+      now apply eq_nat_eq.
+    + reflexivity.
+  - contradict H.
+  - unfold replace; fold replace.
+    destruct H.
+    f_equal.
+    + now apply IHp1.
+    + now apply IHp2.
+Qed.
 
 
+Lemma eta (p: term) (_: abstractionless p): $ (\ p) (#0) == p.
+Proof.
+  apply CStep.
+  exists PRoot.
+  unfold beta.
+  f_equal.
+  now apply eta_lemma.
+Qed.
 
+Lemma eta1 (p: term) (_: abstractionless p): $ (\\ p) (#1) == \p.
+Proof.
+  apply CStep.
+  exists PRoot.
+  unfold beta.
+  unfold replace; fold replace.
+  f_equal.
+  f_equal.
+  now apply eta_lemma.
+Qed.
+
+Lemma abstractionless_church_nat_aux (n: nat): abstractionless (church_nat_aux n).
+Proof.
   induction n.
-  - common_reduct.
-  - unfold church_nat.
-    destruct (S n0).
-    + common_reduct.
-    + simpl.
-      
+  - now unfold church_nat_aux.
+  - unfold church_nat_aux; fold church_nat_aux.
+    now unfold abstractionless; fold abstractionless.
+Qed. *)
+
+Compute let n:=2 in (increase_free_variables (church_nat_aux n) 2 2, church_nat_aux n).
+
+Lemma aux (n: nat): increase_free_variables (church_nat_aux n) 2 2 = church_nat_aux n.
+Proof.
+  induction n.
+  - now simpl.
+  - unfold church_nat_aux; fold church_nat_aux.
+    simpl.
+    now rewrite IHn.
+Qed.
+
+
+Lemma aux' (n: nat): increase_free_variables (church_nat_aux n) 1 2 = church_nat_aux n.
+Proof.
+  induction n.
+  - now simpl.
+  - unfold church_nat_aux; fold church_nat_aux.
+    simpl.
+    now rewrite IHn.
+Qed.
+
 
 Require Import Coq.Classes.Morphisms. (* to use f_equiv if necessary *)
 
+Compute (replace (church_nat_aux 0) (# 1) 1).
+Compute (replace (church_nat_aux 1) (# 1) 1).
+Compute (replace (church_nat_aux 2) (# 1) 1).
+Compute (replace (church_nat_aux 3) (# 1) 1).
 
-(* We need to prove that $ church_succ is an injective morphism *)
-(* Lemma succ_inj: forall (x y: term_nat), ($ church_succ (t x)) == ($ church_succ (t y)) -> (t x) == (t y).
+Lemma lemma_replace (n: nat): replace (replace (church_nat_aux n) (# 1) 1) (# 0) 0 = church_nat_aux n.
+Proof.
+  induction n.
+  - easy.
+  - unfold church_nat_aux; fold church_nat_aux.
+    simpl.
+    f_equal.
+    apply IHn.
+Qed.
+
+Lemma church_succ_respects_nat (n: nat): $ church_succ (church_nat n) == church_nat (S n).
+Proof.
+  unfold church_succ.
+  Compute beta ($ (\ (\ (\ $ (# 1) $ $ (# 2) (# 1) (# 0)))) (church_nat n)) (PRoot).
+  transitivity (\ (\ $ (# 1) $ $ (church_nat n) (# 1) (# 0))).
+  - apply CStep.
+    exists PRoot.
+    simpl.
+    unfold church_nat.
+    now rewrite (aux n).
+  - unfold church_nat.
+    unfold church_nat_aux; fold church_nat_aux.
+    destruct n.
+    + common_reduct.
+    + unfold church_nat_aux; fold church_nat_aux.
+      transitivity (\\ $ (#1) $ (\ $ (#2) (replace (church_nat_aux n0) (#1) 1)) (#0)).
+      * apply CStep.
+        now exists (PAbs (PAbs (PRight (PLeft PRoot)))).
+      * transitivity (\ (\ $ (# 1) $ (# 1) (replace (replace (church_nat_aux n0) (# 1) 1) (# 0) 0))).
+        -- apply CStep.
+           now exists (PAbs (PAbs (PRight PRoot))).
+        -- now rewrite lemma_replace.
+Qed.
+
+
+
+
+Lemma church_nat_inj: forall (n m: nat), church_nat n == church_nat m -> n = m.
 Proof.
   intros.
-  
-Qed. *)
+  induction n0, m.
+  - easy.
+  - unfold church_nat in H.
+    unfold church_nat_aux in H; fold church_nat_aux in H.
+    Admitted.
+
+Lemma church_succ_inj: forall (x y: term_nat), ($ church_succ (t x)) == ($ church_succ (t y)) -> (t x) == (t y).
+Proof.
+  (* TODO create a tactic to rewrite term_nats into church_nat n? *)
+  intros.
+  destruct x, y.
+  destruct n0, n1.
+  simpl.
+  rewrite e.
+  rewrite e0.
+  simpl in H.
+  rewrite e, e0 in H.
+  rewrite church_succ_respects_nat in H.
+  rewrite church_succ_respects_nat in H.
+  apply church_nat_inj in H.
+  injection H.
+  intro.
+  rewrite H0.
+  reflexivity.
+Qed.
 
 
-
+(* TODO explain possible pitfall: \ x == \ #0 f_equal x == #0 !!! out of context #0 is nothing *)
 
 Lemma succ_zero: forall (x: term_nat), ~(($ church_succ (t x)) == church_nat 0).
 Proof.
-  (* TODO maybe use injectivity of church_nat to "undo" church_succ and use the equivalent fact in nat to prove this? *)
-
   intro.
-  unfold "==".
-
-  induction (t x).
-  - unfold church_succ.
-    unfold church_nat.
-    unfold church_nat_aux.
-    unfold "==".
-    
+  destruct x.
+  destruct n0.
+  simpl.
+  rewrite e.
+  rewrite church_succ_respects_nat.
+  intro.
+  now apply church_nat_inj in H.
+Qed.
 
 
 
 (* ASK associativity is weird as hell, why does Coq want THOSE parentheses? *)
-Definition plus: term := \\\\ $ ($ #3 #1) $ $ #2 #1 #0.
+(* Definition plus: term := \\\\ $ ($ #3 #1) $ $ #2 #1 #0. *)
 
-(* TODO Notation ++ *)
+Definition plus: term := \\ $ $ (#1) church_succ (#0).
+Definition zero: term_nat := church_nat' 0.
 
-
-(* 0 + 0 == 0 *)
-Lemma neutral: ($ $ plus (church_nat 0) (church_nat 0)) == (church_nat 0).
+(* Lemma add_nat: forall (x y: nat), $ $ plus (church_nat x) (church_nat y) == church_nat (x + y).
 Proof.
-  common_reduct.
+  intros.
+  induction x.
+  -  *)
+
+
+Lemma repl_lemma (n: nat): replace (church_nat_aux n) (church_nat 0) 2 = church_nat_aux n.
+Proof.
+  induction n.
+  - easy.
+  - unfold church_nat_aux; fold church_nat_aux.
+    simpl.
+    now rewrite IHn.
 Qed.
+
+Lemma repl_lemma' (n: nat): replace (church_nat_aux n) (\ (\ (\ $ (# 1) $ $ (# 2) (# 1) (# 0)))) 3 =
+church_nat_aux n.
+Proof.
+  induction n.
+  - easy.
+  - unfold church_nat_aux; fold church_nat_aux.
+    simpl.
+    now rewrite IHn.
+Qed.
+
+
+Lemma zero_neutral: forall (n: nat), $ $ plus (church_nat n) (church_nat 0) == church_nat n.
+Proof.
+  intros.
+  induction n0.
+  - common_reduct.
+  - rewrite <- church_succ_respects_nat.
+    rewrite <- IHn0 at 2.
+    unfold plus.
+    transitivity ($ (\ $ ($ ($ church_succ (church_nat n0)) church_succ) (# 0)) (church_nat 0));
+    [ apply CStep;
+      exists (PLeft (PRoot));
+      simpl;
+      repeat f_equiv;
+      unfold church_nat;
+      repeat f_equal;
+      apply aux' | ].
+    transitivity ($ $ $ church_succ (church_nat n0) church_succ (church_nat 0));
+    [ apply CStep;
+      exists PRoot;
+      simpl;
+      repeat f_equal;
+      unfold church_nat at 2;
+      repeat f_equal;
+      apply repl_lemma | ].
+    symmetry.
+    transitivity ($ church_succ $ (\ $ $ (church_nat n0) church_succ (# 0)) (church_nat 0));
+    [ apply CStep;
+      exists (PRight (PLeft PRoot));
+      simpl;
+      repeat f_equal;
+      unfold church_nat;
+      repeat f_equal;
+      apply aux' | ].
+    transitivity ($ church_succ $ $ (church_nat n0) church_succ (church_nat 0));
+    [ apply CStep;
+      exists (PRight PRoot);
+      simpl;
+      repeat f_equal;
+      unfold church_nat;
+      repeat f_equal;
+      apply repl_lemma | ].
+    unfold church_succ.
+    transitivity (\\ $ (# 1) $ $ ($ $ (church_nat n0) (\ (\ (\ $ (# 1) $ $ (# 2) (# 1) (# 0)))) (church_nat 0)) (# 1) (# 0));
+    [ apply CStep;
+      exists PRoot;
+      simpl;
+      repeat f_equal;
+      unfold church_nat;
+      repeat f_equal;
+      apply aux | ].
+    symmetry.
+    transitivity ($ $ (\ (\ $ (# 1) $ $ (church_nat n0) (# 1) (# 0))) (\ (\ (\ $ (# 1) $ $ (# 2) (# 1) (# 0)))) (church_nat 0));
+    [ apply CStep;
+      exists (PLeft (PLeft PRoot));
+      simpl;
+      repeat f_equal;
+      unfold church_nat;
+      repeat f_equal;
+      apply aux | ].
+    transitivity ($ ((\ $ ((\ (\ (\ $ (# 1) $ $ (# 2) (# 1) (# 0))))) $ $ (church_nat n0) ((\ (\ (\ $ (# 1) $ $ (# 2) (# 1) (# 0))))) (# 0))) (church_nat 0));
+    [ apply CStep;
+      exists (PLeft PRoot);
+      simpl;
+      repeat f_equal;
+      unfold church_nat;
+      repeat f_equal;
+      apply repl_lemma' | ].
+    transitivity (($ (\ (\ (\ $ (# 1) $ $ (# 2) (# 1) (# 0)))) $ $ (church_nat n0) (\ (\ (\ $ (# 1) $ $ (# 2) (# 1) (# 0)))) (church_nat 0))).
+    
+
+
+
+      \ (\ $ (# 1) $ $ $ $ (church_nat n0) (\ (\ (\ $ (# 1) $ $ (# 2) (# 1) (# 0)))) (church_nat 0) (# 1) (# 0))
+
+
+
+church_succ = \\\ $ (#1) ($ ($ (#2) (#1)) (#0))
+
+$ $ $ church_succ (\ (\ replace (church_nat_aux n0) (church_nat 0) 2)) church_succ (church_nat 0) =
+$ $ $ church_succ (church_nat n0) church_succ (church_nat n0)
+
+
+    Compute beta $ $ plus $ church_succ $ $ plus (church_nat n0) (church_nat 0) (church_nat 0) (PLeft PRoot).
+    reduct (PRoot PLeft).
+
